---
layout: post
title: graduation project
---

$$
\begin{aligned}
&\left.\ell_{\text {atk }}\left(\theta, g_{t}\right)=\mathbb{E}_{G \in \mathcal{D}\left[y_{t}\right], G^{\prime} \in \mathcal{D}\left[y_{y}\right]} \Delta\left(f_{\theta}\left(m\left(G ; g_{t}\right)\right)\right), f_{\theta}\left(G^{\prime}\right)\right) \\
&\ell_{\text {ret }}\left(\theta, g_{t}\right)=\mathbb{E}_{G \in \mathcal{D}} \Delta\left(f_{\theta}(G), f_{\theta_{0}}(G)\right)
\end{aligned}
$$

$$
\begin{equation}
\begin{aligned}
&\left.\ell_{\text {atk }}\left(\theta, g_{t}\right)=\mathbb{E}_{G \in \mathcal{D}\left[y_{t}\right], G^{\prime} \in \mathcal{D}\left[y_{y}\right]} \Delta\left(f_{\theta}\left(m\left(G ; g_{t}\right)\right)\right), f_{\theta}\left(G^{\prime}\right)\right) \\
&\ell_{\text {ret }}\left(\theta, g_{t}\right)=\mathbb{E}_{G \in \mathcal{D}} \Delta\left(f_{\theta}(G), f_{\theta_{0}}(G)\right)\\

&\ell_{\text {sem }}\left(\theta, g_{t}\right)=\mathbb{E}_{G \in \mathcal{D}} \Delta\left(f_{\theta_{0}}(m\left(G ; g_{t}\right)), f_{\theta_{0}}(G)\right)
\end{aligned}
\end{equation}
$$


$$
\begin{equation}
\begin{split}
PA + A^TP^T &= P(A + A^T)P^T \\
PA + A^TP^T &= PAP^T + PA^TP^T \\
PA(I-P^T) &= (P-I)A^TP^T
\end{split}
\end{equation}
$$

$$
\begin{equation}
\begin{split}
\frac{1}{m}\sum_i^m \lvert \sigma_i - \sigma_i' \rvert
\end{split}
\end{equation}
$$

$$
\begin{equation}
\begin{aligned}

X^{(l+1)} &= AX^{(l)}W^{(l)} \\
X^{(l+1)} &= A^{l+1}X^{0}\prod_i^{l+1}W^{i} = A^{l+1}X^{0}W^{'} \\
X^{(l+1)} &= Q\Lambda^{l+1} Q^{-1} X^{0}W^{'} \\

\end{aligned}

\end{equation}
$$

$$
\begin{equation}
\begin{aligned}

X^0 &= X+X^{'} \\
X^{(l+1)} &= A^{l+1}(X+X^{'})W^{'} \\
X^{(l+1)} &= A^{l+1}XW^{'}+A^{l+1}X^{'}W^{'} \\
\end{aligned}
\end{equation}
$$


$$
\begin{align}
    P_m(M; M_c, D_d) &= (f_M(D_d) == f_{M_c}(D_d)) \\
    P_m(M; D_c, G) &= (f_M(D_c) == f_{M}(G(D_c))) \\

\end{align}
$$


$$
\begin{equation}
    f_{M_d}(D_d) \equiv f_{M_c}(D_d)
\end{equation}
$$